WIP ooo_input_top, connected components

dataplane/Examples/Ooo_Input_top.thy
@@ -12,12 +12,17 @@ abbreviation "obtain_progress os \<equiv> (os\<lparr> consu := [], inter := [], 
 abbreviation "drop_cap os cap \<equiv> (os\<lparr> inter := inter os @ [(out cap, time cap, -1)] \<rparr>)"
 abbreviation "drop_caps os caps \<equiv> (os\<lparr> inter := inter os @ map (\<lambda> cap. (out cap, time cap, -1)) caps \<rparr>)"
 abbreviation "mint_cap os p t \<equiv> os\<lparr> inter := inter os @ [(p, t, 1)] \<rparr>"
+
 abbreviation \<open>mint os caps p t \<equiv> if t \<in> set (caps p) then (caps, os) else (caps(p := caps p @ [t]), mint_cap os p t)\<close>
 
 corec ooo_input_top where
   \<open>ooo_input_top os caps ins = choice3
   (Choice (cimage (\<lambda>p. case ins p of
-    LCons (Data t d) lxs \<Rightarrow> Silent (ooo_input_top (produce os (Cap t p) [d]) caps (ins(p := lxs)))
+    LCons (Data t d) lxs \<Rightarrow>
+      let (caps', os') = if lnull lxs
+        then (caps(p := []), drop_caps os (map (\<lambda>t. Cap t p) (caps p)))
+        else (caps, os)
+      in Silent (ooo_input_top (produce os' (Cap t p) [d]) caps' (ins(p := lxs)))
   | LCons (Watermark wm) lxs \<Rightarrow>
       let (caps', os') = mint os caps p wm;
           A = antichain (minimal_antichain (set (caps' p)));
@@ -35,8 +40,10 @@ corec ooo_input_top where
 
 lemma step_ooo_input_top_elim:
   assumes \<open>step io (ooo_input_top os caps ins) op\<close>
-  obtains p t d lxs where \<open>io = Tau\<close> \<open>ins p = LCons (Data t d) lxs\<close>
-    \<open>op = ooo_input_top (produce os (Cap t p) [d]) caps (ins(p := lxs))\<close> \<open>p \<notin> defaults\<close>
+  obtains p t d lxs caps' os' where \<open>io = Tau\<close> \<open>ins p = LCons (Data t d) lxs\<close>
+    \<open>(caps', os') = (if lnull lxs then (caps(p := []), drop_caps os (map (\<lambda>t. Cap t p) (caps p)))
+      else (caps, os))\<close>
+    \<open>op = ooo_input_top (produce os' (Cap t p) [d]) caps' (ins(p := lxs))\<close> \<open>p \<notin> defaults\<close>
   | p wm lxs caps' os' A dropped_caps caps'' os'' where \<open>io = Tau\<close> \<open>ins p = LCons (Watermark wm) lxs\<close>
     \<open>(caps', os') = mint os caps p wm\<close> \<open>A = antichain (minimal_antichain (set (caps' p)))\<close>
     \<open>dropped_caps = map (\<lambda>t. Cap t p) (filter (if lnull lxs then \<top> else Not \<circ> frontier_less_equal A) (caps' p))\<close>
@@ -65,8 +72,10 @@ lemma step_ooo_input_top_Write_None[intro]:
   by (subst ooo_input_top.code) auto
 
 lemma step_ooo_input_top_Silent_Data[intro]:
-  \<open>ins p = LCons (Data t d) lxs \<Longrightarrow> op = ooo_input_top (produce os (Cap t p) [d]) caps (ins(p := lxs)) \<Longrightarrow>
-  p \<notin> defaults \<Longrightarrow> step Tau (ooo_input_top os caps ins) op\<close>
+  \<open>ins p = LCons (Data t d) lxs \<Longrightarrow>
+  (caps', os') = (if lnull lxs then (caps(p := []), drop_caps os (map (\<lambda>t. Cap t p) (caps p))) else (caps, os)) \<Longrightarrow>
+  op = ooo_input_top (produce os' (Cap t p) [d]) caps' (ins(p := lxs)) \<Longrightarrow> p \<notin> defaults \<Longrightarrow>
+  step Tau (ooo_input_top os caps ins) op\<close>
   by (subst ooo_input_top.code) fastforce
 
 lemma step_ooo_input_top_Silent_Watermark[intro]:
@@ -84,10 +93,6 @@ lemma snd_foldl:
   \<open>snd (foldl (\<lambda>(a, b) x. (f a b x, g b x)) (a, b) xs) = foldl g b xs\<close>
   by (induction xs arbitrary: a b) simp_all
 
-lemma foldl_id2:
-  \<open>foldl (\<lambda>x y. x) x xs = x\<close>
-  by (induction xs) simp_all
-
 abbreviation ooo_input_os_caps_Watermark where
   \<open>ooo_input_os_caps_Watermark p wm os caps \<equiv>
   (let (caps', os') = mint os caps p wm;
@@ -95,75 +100,67 @@ abbreviation ooo_input_os_caps_Watermark where
        dropped_caps = map (\<lambda>t. Cap t p) (filter (Not \<circ> frontier_less_equal A) (caps' p));
        caps'' = caps'(p := filter (frontier_less_equal A) (caps' p));
        os'' = drop_caps os' dropped_caps
-  in (os'', caps''))\<close>
+  in (caps'', os''))\<close>
 
 lemma step_Taus_ooo_input_top:
   \<open>lfinite (ltakeWhile (Not \<circ> is_Data) (ins p)) \<Longrightarrow>
   ldropWhile (Not \<circ> is_Data) (ins p) = LCons (Data t d) lxs \<Longrightarrow>
-  (os', caps') = foldl (\<lambda>(os, caps) wm. ooo_input_os_caps_Watermark p wm os caps)
-    (os, caps) (list_of (lmap event.time (ltakeWhile (Not \<circ> is_Data) (ins p)))) \<Longrightarrow>
-  os'' = produce os' (Cap t p) [d] \<Longrightarrow> op = ooo_input_top os'' caps' (ins(p := lxs)) \<Longrightarrow> p \<notin> defaults \<Longrightarrow>
+  (caps', os') = foldl (\<lambda>(caps, os) wm. ooo_input_os_caps_Watermark p wm os caps)
+    (caps, os) (list_of (lmap event.time (ltakeWhile (Not \<circ> is_Data) (ins p)))) \<Longrightarrow>
+  (caps'', os'') = (if lnull lxs then (caps'(p := []), drop_caps os' (map (\<lambda>t. Cap t p) (caps' p))) else (caps', os')) \<Longrightarrow>
+  os''' = produce os'' (Cap t p) [d] \<Longrightarrow> op = ooo_input_top os''' caps'' (ins(p := lxs)) \<Longrightarrow> p \<notin> defaults \<Longrightarrow>
   (step Tau)\<^sup>*\<^sup>* (ooo_input_top os caps ins) op\<close>
 proof (induction \<open>ltakeWhile (Not \<circ> is_Data) (ins p)\<close> arbitrary: ins os caps rule: lfinite_induct)
   case LNil
-  hence \<open>ldropWhile (Not \<circ> is_Data) (ins p) = ins p\<close>
-    using ldropWhile_LCons ldropWhile_LNil llist.sel(1) lnull_def ltakeWhile_eq_LNil_iff neq_LNil_conv
+  have \<open>ldropWhile (Not \<circ> is_Data) (ins p) = ins p\<close>
+    using LNil(1) ldropWhile_LCons ldropWhile_LNil llist.sel(1) lnull_def ltakeWhile_eq_LNil_iff neq_LNil_conv
     by (metis (no_types, opaque_lifting))
-  hence \<open>step Tau (ooo_input_top os caps ins)
-  (ooo_input_top (produce os (Cap t p) [d]) caps (ins(p := lxs)))\<close>
-    using LNil step_ooo_input_top_Silent_Data by auto
   thus ?case
-    using LNil by (auto simp add: lnull_def)
+    using LNil(2-) step_ooo_input_top_Silent_Data by auto
 next
   case LCons
-  then show ?case
-  proof -
-    obtain wm where 1: \<open>lhd (ins p) = Watermark wm\<close> \<open>ins p = LCons (Watermark wm) (ltl (ins p))\<close>
-      using LCons(2) event.collapse(2) ltakeWhile.disc(1) llist.collapse(2) o_def by metis
-    obtain os1 caps1 where os1_caps1_def: \<open>(os1, caps1) = ooo_input_os_caps_Watermark p wm os caps\<close>
-      by fastforce
-    have \<open>ltl (ltakeWhile (Not \<circ> is_Data) (ins p)) = ltakeWhile (Not \<circ> is_Data) (ltl (ins p))\<close>
-      using LCons(2) lnull_ltakeWhile ltakeWhile.simps(4) by blast
-    moreover have 2: \<open>ldropWhile (Not \<circ> is_Data) (ltl (ins p)) = LCons (Data t d) lxs\<close>
-      using LCons(2,4) ldropWhile_simps(2) lhd_LCons_ltl ltakeWhile.disc(1) by metis
-    moreover have \<open>(os', caps') =
-    foldl (\<lambda>(os, caps) wm. ooo_input_os_caps_Watermark p wm os caps) (os1, caps1)
+  obtain wm where ins_wm: \<open>lhd (ins p) = Watermark wm\<close> \<open>ins p = LCons (Watermark wm) (ltl (ins p))\<close>
+    using LCons(2) event.collapse(2) ltakeWhile.disc(1) llist.collapse(2) o_def by metis
+  obtain caps1 os1 where caps1_os1_def: \<open>(caps1, os1) = ooo_input_os_caps_Watermark p wm os caps\<close>
+    by fastforce
+  have \<open>ltl (ltakeWhile (Not \<circ> is_Data) (ins p)) = ltakeWhile (Not \<circ> is_Data) (ltl (ins p))\<close>
+    using LCons(2) lnull_ltakeWhile ltakeWhile.simps(4) by blast
+  moreover have ltl_ins_Data: \<open>ldropWhile (Not \<circ> is_Data) (ltl (ins p)) = LCons (Data t d) lxs\<close>
+    using LCons(2,4) ldropWhile_simps(2) lhd_LCons_ltl ltakeWhile.disc(1) by metis
+  moreover have \<open>(caps', os') =
+    foldl (\<lambda>(caps, os) wm. ooo_input_os_caps_Watermark p wm os caps) (caps1, os1)
      (list_of (lmap event.time (ltakeWhile (Not \<circ> is_Data) (ltl (ins p)))))\<close>
-    proof -
-      have \<open>(os', caps') = foldl (\<lambda>(os, caps) wm. ooo_input_os_caps_Watermark p wm os caps)
-  (os, caps) (wm # list_of (lmap event.time (ltakeWhile (Not \<circ> is_Data) (ltl (ins p)))))\<close>
-        using LCons(1,2,5) 1 lhd_LCons_ltl ltakeWhile.ctr(2) by fastforce
-      thus ?thesis
-        by (simp add: os1_caps1_def)
-    qed
-    ultimately have \<open>(step Tau)\<^sup>*\<^sup>* (ooo_input_top os1 caps1 (ins(p := ltl (ins p)))) op\<close>
-      using LCons fun_upd_same fun_upd_upd by (metis (no_types, lifting))
-    moreover have \<open>step Tau (ooo_input_top os caps ins) (ooo_input_top os1 caps1 (ins(p := ltl (ins p))))\<close>
-    proof -
-      obtain caps' os' where caps'_os'_def: \<open>(caps', os') = mint os caps p wm\<close>
-        by fastforce
-      let ?A = \<open>antichain (minimal_antichain (set (caps' p)))\<close>
-      let ?dropped_caps = \<open>map (\<lambda>t. Cap t p) (filter (if lnull (ltl (ins p)) then \<top> else Not \<circ> frontier_less_equal ?A) (caps' p))\<close>
-      have \<open>caps1 = caps'(p := filter (if lnull (ltl (ins p)) then \<bottom> else frontier_less_equal ?A) (caps' p))\<close>
-        using os1_caps1_def caps'_os'_def 2 eq_LConsD ldropWhile_LNil lnull_def prod.simps(1,2)
-        by (smt (verit, best))
-      moreover have \<open>os1 = drop_caps os' ?dropped_caps\<close>
-        using os1_caps1_def caps'_os'_def 2 eq_LConsD ldropWhile_LNil lnull_def
-          operator_state.fold_congs(2) prod.case_eq_if prod.sel(1) snd_eqD
-        by (smt (verit))
-      ultimately show ?thesis
-        using step_ooo_input_top_Silent_Watermark[of ins p wm \<open>ltl (ins p)\<close> caps' os' caps os ?A ?dropped_caps caps1 os1]
-          LCons(8) 1 by (auto simp add: os1_caps1_def caps'_os'_def)
-    qed
-    ultimately show ?thesis
-      using transitive_closurep_trans'(6) by (metis (no_types, lifting))
+  proof -
+    have \<open>(caps', os') = foldl (\<lambda>(caps, os) wm. ooo_input_os_caps_Watermark p wm os caps)
+  (caps, os) (wm # list_of (lmap event.time (ltakeWhile (Not \<circ> is_Data) (ltl (ins p)))))\<close>
+      using LCons(1,2,5) ins_wm(1) lhd_LCons_ltl ltakeWhile.ctr(2) by fastforce
+    thus ?thesis
+      using caps1_os1_def by simp
   qed
+  ultimately have \<open>(step Tau)\<^sup>*\<^sup>* (ooo_input_top os1 caps1 (ins(p := ltl (ins p)))) op\<close>
+    using LCons(3,6,7-9) fun_upd_same fun_upd_upd by (smt (verit, best))
+  moreover have \<open>step Tau (ooo_input_top os caps ins) (ooo_input_top os1 caps1 (ins(p := ltl (ins p))))\<close>
+  proof -
+    obtain caps' os' where caps'_os'_def: \<open>(caps', os') = mint os caps p wm\<close> by fastforce
+    let ?A = \<open>antichain (minimal_antichain (set (caps' p)))\<close>
+    let ?dropped_caps = \<open>map (\<lambda>t. Cap t p) (filter (if lnull (ltl (ins p)) then \<top> else Not \<circ> frontier_less_equal ?A) (caps' p))\<close>
+    have \<open>caps1 = caps'(p := filter (if lnull (ltl (ins p)) then \<bottom> else frontier_less_equal ?A) (caps' p))\<close>
+      using caps1_os1_def caps'_os'_def ltl_ins_Data eq_LConsD ldropWhile_LNil lnull_def prod.simps(1,2)
+      by (smt (verit, best))
+    moreover have \<open>os1 = drop_caps os' ?dropped_caps\<close>
+      using caps1_os1_def caps'_os'_def ltl_ins_Data eq_LConsD ldropWhile_LNil lnull_def
+        operator_state.fold_congs(2) prod.case_eq_if prod.sel(1) snd_eqD
+      by (smt (verit))
+    ultimately show ?thesis
+      using LCons(9) ins_wm(2) caps'_os'_def by blast
+  qed
+  ultimately show ?case
+    using transitive_closurep_trans'(6) by (metis (no_types, lifting))
 qed
 
-lemma outpu_fst_foldl_ooo_input_os_caps_Watermark_Nil:
+lemma outpu_snd_foldl_ooo_input_os_caps_Watermark_Nil:
   \<open>outpu os p = [] \<Longrightarrow>
-  outpu (fst (foldl (\<lambda>(os, caps) wm. (ooo_input_os_caps_Watermark p wm os caps))
-    (os, caps) lxs)) p = []\<close>
+  outpu (snd (foldl (\<lambda>(caps, os) wm. (ooo_input_os_caps_Watermark p wm os caps)) (caps, os) lxs)) p = []\<close>
   by (induction lxs arbitrary: os caps) simp_all
 
 abbreviation ooo_inp_op where
@@ -199,7 +196,7 @@ proof (coinduction arbitrary: sg os caps ins rule: wbisim_coinduct_upto'')
        apply (rule rtranclp.intros(1))
       apply (rule wbc_base)
       apply (intro exI conjI)
-        apply (auto intro: arg_cong[where ?f=\<open>map_op (Pair 0) (Pair 0)\<close>] arg_cong[where ?f=source_op] simp add: produce_def)
+        apply (auto intro: arg_cong[where f=\<open>map_op (Pair 0) (Pair 0)\<close>] arg_cong[where f=source_op] simp add: produce_def split: if_splits)
       done
     subgoal
       apply (intro exI conjI)
@@ -207,7 +204,7 @@ proof (coinduction arbitrary: sg os caps ins rule: wbisim_coinduct_upto'')
       apply (rule wbc_base)
       apply (intro exI conjI)
         apply (rule refl)
-       apply (auto intro: arg_cong[where ?f=\<open>map_op (Pair 0) (Pair 0)\<close>] arg_cong[where ?f=source_op] simp add: produce_def split: if_splits)
+       apply (auto intro: arg_cong[where f=\<open>map_op (Pair 0) (Pair 0)\<close>] arg_cong[where f=source_op] simp add: produce_def split: if_splits)
       done
     subgoal
       apply (intro exI conjI[rotated, OF wbc_base])
@@ -238,17 +235,17 @@ next
          apply (rule step_map_op)
           apply (rule step_ooo_input_top_Write_Some)
             apply (simp_all add: produce_def)
-         apply (drule outpu_fst_foldl_ooo_input_os_caps_Watermark_Nil)
+         apply (drule outpu_snd_foldl_ooo_input_os_caps_Watermark_Nil)
          apply fastforce
         apply (rule wbc_base)
         apply (intro exI conjI)
           apply (rule refl)
-         apply (auto intro!: arg_cong[where ?f=\<open>map_op (Pair 0) (Pair 0)\<close>] arg_cong[where ?f=source_op] simp add: foldl_id2 fun_eq_iff)
+         apply (auto intro!: arg_cong[where f=\<open>map_op (Pair 0) (Pair 0)\<close>] arg_cong[where f=source_op] simp add: fun_eq_iff)
         using ltl_lfilter ext comp_apply ltl_lmap ltl_simps(2) apply (metis (lifting))
         done
       subgoal
         apply (intro exI conjI[rotated, OF wbc_base])
-         apply (auto intro!: arg_cong[where ?f=\<open>map_op (Pair 0) (Pair 0)\<close>] arg_cong[where ?f=source_op])
+         apply (auto intro!: arg_cong[where f=\<open>map_op (Pair 0) (Pair 0)\<close>] arg_cong[where f=source_op])
         done
       done
     done
