dataplane/Examples/ConnectedComponents.thy
@@ -54,11 +54,16 @@ primrec list_span where
   \<open>list_span _ [] = ([], [])\<close>
 | \<open>list_span P (x # xs) = (let (ys, zs) = list_span P xs in if P x then (x # ys, zs) else ([], xs))\<close>
 
-function group_by where
+lemma list_span_length_le[termination_simp]:
+  \<open>(ys, zs) = list_span P xs \<Longrightarrow> length ys \<le> length xs\<close>
+  \<open>(ys, zs) = list_span P xs \<Longrightarrow> length zs \<le> length xs\<close>
+  by (induction xs arbitrary: ys zs) (auto split: if_splits prod.splits)
+
+fun group_by where
   \<open>group_by _ [] = []\<close>
 | \<open>group_by f (x # xs) = (let (ys, zs) = list_span (f x) xs in (x # ys) # (group_by f zs))\<close>
-  by auto (meson list.exhaust)
 
+(*
 primrec remdups_f where
   \<open>remdups_f f [] = []\<close>
 | \<open>remdups_f f (x # xs) = (if f x \<in> f ` set xs then remdups_f f xs else x # remdups_f f xs)\<close>
@@ -94,6 +99,7 @@ lemma distinct_remdups_f_id:
 lemma remdups_f_id_iff_distinct[simp]:
   \<open>remdups_f f xs = xs \<longleftrightarrow> distinct (map f xs)\<close>
   by (metis distinct_map_remdups_f distinct_remdups_f_id)
+*)
 
 definition insort_union where
   \<open>insort_union = fold insort_insert\<close>
@@ -119,43 +125,44 @@ definition update_label :: \<open>('t \<Rightarrow> 'v :: linorder \<Rightarrow>
   (let f = if is_Nil tis then label t else unions_with min (map label tis)
   in label(t := f(b := min (f b) a)))\<close>
 
-(* TODO Define proper condition for outputting (check frontier and convergence of the label propagation. *)
+(* TODO Check minting of capabilities, on proper ports. *)
+(* TODO Finish definition when checking the frontiers (before outputting). *)
 declare [[unify_search_bound = 420]]
 corec label_prop_op where
   \<open>label_prop_op os caps tis G vs label = choice6
   (Read None (\<lambda>st. case st of Inl (Inr f) \<Rightarrow> label_prop_op (os\<lparr>front := f\<rparr>) caps tis G vs label | _ \<Rightarrow> \<oslash>))
   (Read (Some (0 :: 2)) (\<lambda>x. case x of
     Inr (Inr (s, d), t) \<Rightarrow>
-      let (caps', os') = mint os caps 0 t;
+      let t1 = myfst t;
+          t' = MyPair t1 0;
+          (caps', os') = if t1 \<in> set (map myfst (caps (0 :: 1))) then (caps, os) else (caps(0 := caps 0 @ [t']), mint_cap os 0 t');
           os'' = consume os' 0 t 1;
-          t1 = myfst t;
           G' = G(t1 := (G t1)(s := List.insert d (G t1 s), d := List.insert s (G t1 d)));
           (a, b) = (min s d, max s d);
           label' = update_label label a b t1 (filter ((\<le>) t1) tis);
           bs = neighbors G' t1 (filter ((\<le>) t1) tis) b;
           batch = if label t1 b > a
-            then map (\<lambda>v. (Inr (v, a), Cap t 0)) (filter (\<lambda>v. label t1 v > a) bs)
+            then map (\<lambda>v. (Inr (v, a), Cap t 1)) (filter (\<lambda>v. label t1 v > a) bs)
             else [];
           os''' = produces os'' batch
      in label_prop_op os''' caps' (List.insert t1 tis) G' (insort_union [s, d] vs) label'
   | _ \<Rightarrow> \<oslash>))
   (Read (Some (1 :: 2)) (\<lambda>x. case x of
     Inr (Inr (n, x), t) \<Rightarrow>
-      let (caps', os') = mint os caps 0 t;
-          (caps'', os'') = mint os' caps' 1 t;
-          os''' = consume os'' 1 t 1;
+      let os' = consume os 1 t 1;
           t1 = myfst t;
           label' = update_label label x n t1 (filter ((\<le>) t1) tis);
           ns = neighbors G t1 (filter ((\<le>) t1) tis) n;
           batch = if label t1 n > x
-            then map (\<lambda>v. (Inr (v, x), Cap t 0)) (filter (\<lambda>v. label t1 v > x) ns)
+            then map (\<lambda>v. (Inr (v, x), Cap t 1)) (filter (\<lambda>v. label t1 v > x) ns)
             else [];
-          os'''' = produces os''' batch
-    in label_prop_op os'''' caps'' tis G vs label'
+          os'' = produces os' batch
+    in label_prop_op os'' caps tis G vs label'
   | _ \<Rightarrow> \<oslash>))
-  (let dropped_caps = map (\<lambda>t. Cap t 0) (filter (Not \<circ> frontier_less_equal (front os 0)) (caps 0));
-       caps' = caps(0 := filter (frontier_less_equal (front os 0)) (caps 0));
-       output_caps = sort_key (myfst \<circ> time) (remdups_f (myfst \<circ> time) dropped_caps);
+  (let A = front os 0 + front os 1;
+       dropped_caps = map (\<lambda>t. Cap t 0) (filter undefined (caps 0));
+       caps' = caps(0 := filter undefined (caps 0));
+       output_caps = sort_key (myfst \<circ> time) dropped_caps;
        batch = map (\<lambda>cap. let t = myfst (time cap) in
         (Inl (group_by (\<lambda>v u. label t v = label t u) vs), cap)) output_caps;
        os' = produces os batch;
@@ -179,8 +186,14 @@ abbreviation label_op where
 
 abbreviation incr_op' where
   \<open>incr_op' incr os \<equiv>
-  map_op (case_option (Inl (2 :: 3)) (\<lambda>p. Inr (1, p))) (case_option (Inl (2 :: 3)) (\<lambda>p. Inr (2, p)))
+  map_op (case_option (Inl (2 :: 3)) (\<lambda>p. Inr (2, p))) (case_option (Inl (2 :: 3)) (\<lambda>p. Inr (2, p)))
   (increment_top incr os)\<close>
+
+(* Issue: I would like to consider the input and increment operators with only 1 input port and 1
+output port, however this is not possible here because the numeral type 2 for ports is the same for
+all operators in the graph.  I cannot use map_op to solve this issue because the type parameter for
+ports occurs inside the shared_state type, which occurs inside the type of data for the operators,
+and this is a dead type parameter. *)
 
 abbreviation label_incr_op where
   \<open>label_incr_op os1 caps tis G vs label buf incr os2 \<equiv>
@@ -205,6 +218,7 @@ abbreviation cc_edges where
   else if l = Loc 2 (Src 0) then [Loc 1 (Trg 1)]
   else [])\<close>
 
+(* Note: I omit some internal connections of the input and increment operators. *)
 abbreviation cc_summary where
   \<open>cc_summary \<equiv> (\<lambda>l1 l2.
   if l1 = Loc (0 :: 3) (Trg (0 :: 2)) \<and> l2 = Loc (0 :: 3) (Src (0 :: 2))
@@ -213,6 +227,10 @@ abbreviation cc_summary where
   then antichain {0}
   else if l1 = Loc 1 (Trg 0) \<and> l2 = Loc 1 (Src 0)
   then antichain {0}
+  else if l1 = Loc 1 (Trg 0) \<and> l2 = Loc 1 (Src 1)
+  then antichain {0}
+  else if l1 = Loc 1 (Trg 1) \<and> l2 = Loc 1 (Src 0)
+  then antichain {0}
   else if l1 = Loc 1 (Trg 1) \<and> l2 = Loc 1 (Src 1)
   then antichain {0}
   else if l1 = Loc 1 (Src 1) \<and> l2 = Loc 2 (Trg 0)
@@ -220,6 +238,6 @@ abbreviation cc_summary where
   else if l1 = Loc 2 (Trg 0) \<and> l2 = Loc 2 (Src 0)
   then antichain {0}
   else if l1 = Loc 2 (Src 0) \<and> l2 = Loc 1 (Trg 1)
-  then antichain {0}
+  then antichain {MyPair 0 1}
   else {}\<^sub>A)\<close>
 end
